Improve branch tunneling
The previous branch tunneling was missing optimization opportunities
introduced by the optimization of conditional branches.  For example:

L1: instr; branch L2
L2: if cond then branch L3 else branch L4
L3: branch L4
L4: ...

was transformed into

L1: instr; branch L2
L2: branch L4
L3: branch L4
L4: ...

missing a tunneling opportunity (branch L2 -> branch L4).

This commit improves branch tunneling so that the expected code is produced:

L1: instr; branch L4
L2: branch L4
L3: branch L4
L4: ...

To this end, additional equalities are introduced in the union-find
data structure corresponding to optimizable conditional branches.

In rare cases these additional equalities trigger new opportunities for
optimizing conditional branches.  Hence we iterate the analysis
until no optimizable conditional branch remains.

backend/Tunnelingproof.v
@@ -12,6 +12,7 @@
 
 (** Correctness proof for the branch tunneling optimization. *)
 
+Require Import FunInd.
 Require Import Coqlib Maps UnionFind.
 Require Import AST Linking.
 Require Import Values Memory Events Globalenvs Smallstep.
@@ -29,12 +30,21 @@ Qed.
 
 (** * Properties of the branch map computed using union-find. *)
 
-Definition measure_edge (u: U.t) (pc s: node) (f: node -> nat) : node -> nat :=
+Section BRANCH_MAP_CORRECT.
+
+Variable fn: LTL.function.
+
+Definition measure_branch (u: U.t) (pc s: node) (f: node -> nat) : node -> nat :=
   fun x => if peq (U.repr u s) pc then f x
            else if peq (U.repr u x) pc then (f x + f s + 1)%nat
            else f x.
 
-Definition branch_map_correct (c: code) (u: U.t) (f: node -> nat): Prop :=
+Definition measure_cond (u: U.t) (pc s1 s2: node) (f: node -> nat) : node -> nat :=
+  fun x => if peq (U.repr u s1) pc then f x
+           else if peq (U.repr u x) pc then (f x + Nat.max (f s1) (f s2) + 1)%nat
+           else f x.
+
+Definition branch_map_correct_1 (c: code) (u: U.t) (f: node -> nat): Prop :=
   forall pc,
   match c!pc with
   | Some(Lbranch s :: b) =>
@@ -43,58 +53,208 @@ Definition branch_map_correct (c: code) (u: U.t) (f: node -> nat): Prop :=
       U.repr u pc = pc
   end.
 
-Lemma record_gotos_correct_1:
-  forall fn, { f | branch_map_correct fn.(fn_code) (record_gotos fn) f }.
+Lemma record_branch_correct:
+  forall c u f pc b,
+  branch_map_correct_1 (PTree.remove pc c) u f ->
+  c!pc = Some b ->
+  { f' | branch_map_correct_1 c (record_branch u pc b) f' }.
 Proof.
-  intros.
-  unfold record_gotos. apply PTree_Properties.fold_ind.
-
-- (* base case *)
-  intros m EMPTY. exists (fun _ => O). 
-  red; intros. rewrite EMPTY. apply U.repr_empty.
-
-- (* inductive case *)
-  intros m u pc bb GET1 GET2 [f BMC].
+  intros c u f pc b BMC GET1.
   assert (PC: U.repr u pc = pc).
   { specialize (BMC pc). rewrite PTree.grs in BMC. auto. }
-  assert (DFL: { f | branch_map_correct m u f }).
+  assert (DFL: { f | branch_map_correct_1 c u f }).
   { exists f. intros p. destruct (peq p pc).
-  - subst p. rewrite GET1. destruct bb as [ | [] bb ]; auto.
+  - subst p. rewrite GET1. destruct b as [ | [] b ]; auto.
   - specialize (BMC p). rewrite PTree.gro in BMC by auto. exact BMC.
   }
-  unfold record_goto. destruct bb as [ | [] bb ]; auto.
-  exists (measure_edge u pc s f). intros p. destruct (peq p pc).
-+ subst p. rewrite GET1. unfold measure_edge.
+  unfold record_branch. destruct b as [ | [] b ]; auto.
+  exists (measure_branch u pc s f). intros p. destruct (peq p pc).
++ subst p. rewrite GET1. unfold measure_branch.
   rewrite (U.repr_union_2 u pc s); auto. rewrite U.repr_union_3.
   destruct (peq (U.repr u s) pc); auto. rewrite PC, peq_true. right; split; auto. lia.
 + specialize (BMC p). rewrite PTree.gro in BMC by auto.
   assert (U.repr u p = p -> U.repr (U.union u pc s) p = p).
   { intro. rewrite <- H at 2. apply U.repr_union_1. congruence. }
-  destruct (m!p) as [ [ | [] b ] | ]; auto.
+  destruct (c!p) as [ [ | [] _ ] | ]; auto.
   destruct BMC as [A | [A B]]. auto.
   right; split. apply U.sameclass_union_2; auto.
-  unfold measure_edge. destruct (peq (U.repr u s) pc). auto.
+  unfold measure_branch. destruct (peq (U.repr u s) pc). auto.
   rewrite A. destruct (peq (U.repr u s0) pc); lia.
 Qed.
 
-Definition branch_target (f: function) (pc: node) : node :=
-  U.repr (record_gotos f) pc.
+Lemma record_branches_correct:
+  { f | branch_map_correct_1 fn.(fn_code) (record_branches fn) f }.
+Proof.
+  unfold record_branches. apply PTree_Properties.fold_ind.
+- (* base case *)
+  intros m EMPTY. exists (fun _ => O). 
+  red; intros. rewrite EMPTY. apply U.repr_empty.
+- (* inductive case *)
+  intros m u pc bb GET1 GET2 [f BMC]. eapply record_branch_correct; eauto.
+Qed.
 
-Definition count_gotos (f: function) (pc: node) : nat :=
-  proj1_sig (record_gotos_correct_1 f) pc.
+Definition branch_map_correct_2 (c: code) (u: U.t) (f: node -> nat): Prop :=
+  forall pc,
+  match fn.(fn_code)!pc with
+  | Some(Lbranch s :: b) =>
+      U.repr u pc = pc \/ (U.repr u pc = U.repr u s /\ f s < f pc)%nat
+  | Some(Lcond cond args s1 s2 :: b) =>
+      U.repr u pc = pc \/ (c!pc = None /\ U.repr u pc = U.repr u s1 /\ U.repr u pc = U.repr u s2 /\ f s1 < f pc /\ f s2 < f pc)%nat
+  | _ =>
+      U.repr u pc = pc
+  end.
+
+Lemma record_cond_correct:
+  forall c u changed f pc b,
+  branch_map_correct_2 c u f ->
+  fn.(fn_code)!pc = Some b ->
+  c!pc <> None ->
+  let '(c1, u1, _) := record_cond (c, u, changed) pc b in
+  { f' | branch_map_correct_2 c1 u1 f' }.
+Proof.
+  intros c u changed f pc b BMC GET1 GET2.
+  assert (DFL: { f' | branch_map_correct_2 c u f' }).
+  { exists f; auto. }
+  unfold record_cond. destruct b as [ | [] b ]; auto.
+  destruct (peq (U.repr u s1) (U.repr u s2)); auto.
+  exists (measure_cond u pc s1 s2 f).
+  assert (PC: U.repr u pc = pc).
+  { specialize (BMC pc). rewrite GET1 in BMC. intuition congruence. }
+  intro p. destruct (peq p pc).
+- subst p. rewrite GET1. unfold measure_cond.
+  rewrite U.repr_union_2 by auto. rewrite <- e, PC, peq_true.
+  destruct (peq (U.repr u s1) pc); auto.
+  right; repeat split.
+  + apply PTree.grs.
+  + rewrite U.repr_union_3. auto.
+  + rewrite U.repr_union_1 by congruence. auto.
+  + lia.
+  + lia.
+- assert (P: U.repr u p = p -> U.repr (U.union u pc s1) p = p).
+  { intros. rewrite U.repr_union_1 by congruence. auto. }
+  specialize (BMC p). destruct (fn_code fn)!p as [ [ | [] bb ] | ]; auto.
+  + destruct BMC as [A | (A & B)]; auto. right; split.
+    * apply U.sameclass_union_2; auto.
+    * unfold measure_cond. rewrite <- A.
+      destruct (peq (U.repr u s1) pc). auto.
+      destruct (peq (U.repr u p) pc); lia.
+  + destruct BMC as [A | (A & B & C & D & E)]; auto. right; split; [ | split; [ | split]].
+    * rewrite PTree.gro by auto. auto.
+    * apply U.sameclass_union_2; auto.
+    * apply U.sameclass_union_2; auto.
+    * unfold measure_cond. rewrite <- B, <- C.
+      destruct (peq (U.repr u s1) pc). auto.
+      destruct (peq (U.repr u p) pc); lia.
+Qed.
+
+Definition code_compat (c: code) : Prop :=
+  forall pc b, c!pc = Some b -> fn.(fn_code)!pc = Some b.
+
+Definition code_invariant (c0 c1 c2: code) : Prop :=
+  forall pc, c0!pc = None -> c1!pc = c2!pc.
+
+Lemma record_conds_1_correct:
+  forall c u f,
+  branch_map_correct_2 c u f ->
+  code_compat c ->
+  let '(c', u', _) := record_conds_1 (c, u) in
+  (code_compat c' * { f' | branch_map_correct_2 c' u' f' })%type.
+Proof.
+  intros c0 u0 f0 BMC0 COMPAT0.
+  unfold record_conds_1.
+  set (x := PTree.fold record_cond c0 (c0, u0, false)).
+  set (P := fun (cd: code) (cuc: code * U.t * bool) =>
+            (code_compat (fst (fst cuc)) *
+             code_invariant cd (fst (fst cuc)) c0 *
+             { f | branch_map_correct_2 (fst (fst cuc)) (snd (fst cuc)) f })%type).
+  assert (REC: P c0 x).
+  { unfold x; apply PTree_Properties.fold_ind.
+  - intros cd EMPTY. split; [split|]; simpl.
+    + auto.
+    + red; auto.
+    + exists f0; auto.
+  - intros cd [[c u] changed] pc b GET1 GET2 [[COMPAT INV] [f BMC]]. simpl in *.
+    split; [split|].
+    + unfold record_cond; destruct b as [ | [] b]; simpl; auto.
+      destruct (peq (U.repr u s1) (U.repr u s2)); simpl; auto.
+      red; intros. rewrite PTree.grspec in H. destruct (PTree.elt_eq pc0 pc). discriminate. auto.
+    + assert (DFL: code_invariant cd c c0).
+      { intros p GET. apply INV. rewrite PTree.gro by congruence. auto. }
+      unfold record_cond; destruct b as [ | [] b]; simpl; auto.
+      destruct (peq (U.repr u s1) (U.repr u s2)); simpl; auto.
+      intros p GET. rewrite PTree.gro by congruence. apply INV. rewrite PTree.gro by congruence. auto.
+    + assert (GET3: c!pc = Some b).
+      { rewrite <- GET2. apply INV. apply PTree.grs. }
+      assert (X: fn.(fn_code)!pc = Some b) by auto.
+      assert (Y: c!pc <> None) by congruence.
+      generalize (record_cond_correct c u changed f pc b BMC X Y).
+      destruct (record_cond (c, u, changed) pc b) as [[c1 u1] changed1]; simpl.
+      auto.
+  }
+  destruct x as [[c1 u1] changed1]; destruct REC as [[COMPAT1 INV1] BMC1]; auto.
+Qed.
+
+Definition branch_map_correct (u: U.t) (f: node -> nat): Prop :=
+  forall pc,
+  match fn.(fn_code)!pc with
+  | Some(Lbranch s :: b) =>
+      U.repr u pc = pc \/ (U.repr u pc = U.repr u s /\ f s < f pc)%nat
+  | Some(Lcond cond args s1 s2 :: b) =>
+      U.repr u pc = pc \/ (U.repr u pc = U.repr u s1 /\ U.repr u pc = U.repr u s2 /\ f s1 < f pc /\ f s2 < f pc)%nat
+  | _ =>
+      U.repr u pc = pc
+  end.
+
+Lemma record_conds_correct:
+  forall cu,
+  { f | branch_map_correct_2 (fst cu) (snd cu) f } ->
+  code_compat (fst cu) ->
+  { f | branch_map_correct (record_conds cu) f }.
+Proof.
+  intros cu0. functional induction (record_conds cu0); intros.
+- destruct cu as [c u], cu' as [c' u'], H as [f BMC]. 
+  generalize (record_conds_1_correct c u f BMC H0).
+  rewrite e. intros [U V]. apply IHt; auto.
+- destruct cu as [c u], H as [f BMC].
+  exists f. intros pc. specialize (BMC pc); simpl in *.
+  destruct (fn_code fn)!pc as [ [ | [] b ] | ]; tauto.
+Qed.
+
+Lemma record_gotos_correct_1:
+  { f | branch_map_correct (record_gotos fn) f }.
+Proof.
+  apply record_conds_correct; simpl.
+- destruct record_branches_correct as [f BMC].
+  exists f. intros pc. specialize (BMC pc); simpl in *.
+  destruct (fn_code fn)!pc as [ [ | [] b ] | ]; auto.
+- red; auto.
+Qed.
+
+Definition branch_target  (pc: node) : node :=
+  U.repr (record_gotos fn) pc.
+
+Definition count_gotos (pc: node) : nat :=
+  proj1_sig record_gotos_correct_1 pc.
 
 Theorem record_gotos_correct:
-  forall f pc,
-  match f.(fn_code)!pc with
+  forall pc,
+  match fn.(fn_code)!pc with
   | Some(Lbranch s :: b) =>
-       branch_target f pc = pc \/
-       (branch_target f pc = branch_target f s /\ count_gotos f s < count_gotos f pc)%nat
-  | _ => branch_target f pc = pc
+      branch_target pc = pc \/
+      (branch_target pc = branch_target s /\ count_gotos s < count_gotos pc)%nat
+  | Some(Lcond cond args s1 s2 :: b) =>
+      branch_target pc = pc \/
+      (branch_target pc = branch_target s1 /\ branch_target pc = branch_target s2
+       /\ count_gotos s1 < count_gotos pc /\ count_gotos s2 < count_gotos pc)%nat
+  | _ =>
+      branch_target pc = pc
   end.
 Proof.
-  intros. unfold count_gotos. destruct (record_gotos_correct_1 f) as [m P]; simpl.
+  intros. unfold count_gotos. destruct record_gotos_correct_1 as [f P]; simpl.
   apply P.
 Qed.
+
+End BRANCH_MAP_CORRECT.
 
 (** * Preservation of semantics *)
 
@@ -187,13 +347,21 @@ Inductive match_states: state -> state -> Prop :=
         (MEM: Mem.extends m tm),
       match_states (Block s f sp bb ls m)
                    (Block ts (tunnel_function f) sp (tunneled_block f bb) tls tm)
-  | match_states_interm:
+  | match_states_interm_branch:
       forall s f sp pc bb ls m ts tls tm
         (STK: list_forall2 match_stackframes s ts)
         (LS: locmap_lessdef ls tls)
         (MEM: Mem.extends m tm),
       match_states (Block s f sp (Lbranch pc :: bb) ls m)
                    (State ts (tunnel_function f) sp (branch_target f pc) tls tm)
+  | match_states_interm_cond:
+      forall s f sp cond args pc1 pc2 bb ls m ts tls tm
+        (STK: list_forall2 match_stackframes s ts)
+        (LS: locmap_lessdef ls tls)
+        (MEM: Mem.extends m tm)
+        (SAME: branch_target f pc1 = branch_target f pc2),
+      match_states (Block s f sp (Lcond cond args pc1 pc2 :: bb) ls m)
+                   (State ts (tunnel_function f) sp (branch_target f pc1) tls tm)
   | match_states_call:
       forall s f ls m ts tls tm
         (STK: list_forall2 match_stackframes s ts)
@@ -346,6 +514,7 @@ Definition measure (st: state) : nat :=
   match st with
   | State s f sp pc ls m => (count_gotos f pc * 2)%nat
   | Block s f sp (Lbranch pc :: _) ls m => (count_gotos f pc * 2 + 1)%nat
+  | Block s f sp (Lcond _ _ pc1 pc2 :: _) ls m => (Nat.max (count_gotos f pc1) (count_gotos f pc2) * 2 + 1)%nat
   | Block s f sp bb ls m => 0%nat
   | Callstate s f ls m => 0%nat
   | Returnstate s ls m => 0%nat
@@ -380,10 +549,16 @@ Proof.
 
   generalize (record_gotos_correct f pc). rewrite H.
   destruct bb; auto. destruct i; auto.
++ (* Lbranch *)
   intros [A | [B C]]. auto.
   right. split. simpl. lia.
   split. auto.
   rewrite B. econstructor; eauto.
++ (* Lcond *)
+  intros [A | (B & C & D & E)]. auto.
+  right. split. simpl. lia.
+  split. auto.
+  rewrite B. econstructor; eauto. congruence.
 
 - (* Lop *)
   exploit eval_operation_lessdef. apply reglist_lessdef; eauto. eauto. eauto. 
@@ -450,18 +625,24 @@ Proof.
 - (* Lbranch (eliminated) *)
   right; split. simpl. lia. split. auto. constructor; auto.
 
-- (* Lcond *)
+- (* Lcond (preserved) *)
   simpl tunneled_block.
   set (s1 := U.repr (record_gotos f) pc1). set (s2 := U.repr (record_gotos f) pc2).
   destruct (peq s1 s2).
 + left; econstructor; split.
-  eapply exec_Lbranch. 
-  destruct b.
-* constructor; eauto using locmap_undef_regs_lessdef_1.
-* rewrite e. constructor; eauto using locmap_undef_regs_lessdef_1.
+  eapply exec_Lbranch.
+  set (pc := if b then pc1 else pc2).
+  replace s1 with (branch_target f pc) by (unfold pc; destruct b; auto).
+  constructor; eauto using locmap_undef_regs_lessdef_1.
 + left; econstructor; split.
   eapply exec_Lcond; eauto. eapply eval_condition_lessdef; eauto using reglist_lessdef.
   destruct b; econstructor; eauto using locmap_undef_regs_lessdef.
+- (* Lcond (eliminated) *)
+  right; split. simpl. destruct b; lia.
+  split. auto.
+  set (pc := if b then pc1 else pc2).
+  replace (branch_target f pc1) with (branch_target f pc) by (unfold pc; destruct b; auto).
+  econstructor; eauto.
 
 - (* Ljumptable *)
   assert (tls (R arg) = Vint n).
